Updated the Core DKAL engine. Added most of the entails rules and the syntactic (easy) derivation cases.

ModularEngine/src/LogicEngine.FStar/coredkal.fst
@@ -1,21 +1,62 @@
+(************************)
+(* build:               *)
+(* fstar coredkal.fst   *)
+(************************)
+
 module CoreDKAL
 
-type principal = string
-type var = string 
+(********************)
+(* Type definitions *)
+(********************)
 
-type constant = 
-  | Bool : bool -> constant 
-  | Principal : principal -> constant
-  | SubstrateObject : object -> constant 
+(** From types.fst **)
+type principal = string
 
 type typ =  
-    | Boolean : typ
-    | Infon : typ
-    | PrincipalT : typ
-    | SubstrateQuery : typ
-    | Evidence : typ
+  | Infon : typ
+  | Principal : typ
+  | SubstrateUpdate : typ
+  | SubstrateQuery : typ
+  | Action : typ
+  | Condition : typ
+  | RuleT : typ
+  | Evidence : typ
+  | Boolean : typ
+  | Int32 : typ
+  | Double : typ
+  | String : typ
 
-type query 
+type var = string * typ
+  
+type constant = 
+  | True : constant
+  | False : constant
+  (* | Bool : bool -> constant *)
+  | PrincipalConstant : principal -> constant
+  | SubstrateConstant : object -> constant 
+
+type relationInfon
+type func
+
+
+
+
+type substitution
+
+
+type term (*= 
+  | Var : var -> term
+  | Const : constant -> term
+  | Forall : var -> term -> term
+  | App : func -> list term -> term
+  (* | ... *)
+*)
+  
+
+
+(** to be replaced **)
+type query
+
 type evidence =
   | EmptyEv : evidence
   | SigEv : evidence
@@ -26,90 +67,204 @@ type evidence =
 type infon =
   | Variable : var -> infon
 (*   | c  *)
-(*                | forall (x:t). i  *)
+  | Forall : var -> infon -> infon
   | Empty : infon
   | AsInfon : query -> infon
   | And : infon -> infon -> infon
   | Said : infon -> infon -> infon
 (*                | And i j *)
-(*                | Implies i j *)
-
-(*                | Justified i j *)
-
-
+  | Implies : infon -> infon -> infon
+  
+  
+(** added here **)
 type infostrate = list infon
 type substrate = list query
+type varDecl = list var
+type prefix = list infon
+(*
+let said (p:term) (i:term) = App(Said, [p; i])
+*)
+  
+(*************)
+(* Utilities *)
+(*************)
+
+type Mem :: 'a::* => 'a => list 'a => P =
+(* = Inductive definition of list membership in a constructive style *)
+(* look at fine/src/certify/coretyping.fst (module FniteSet for Mem and decideMem) *)
+  | Mem_hd : a:'a -> t:list 'a -> Mem 'a a (a::t)
+  | Mem_tl : a:'a -> h:'a -> t:list 'a -> Mem 'a a t -> Mem 'a a (h::t)
+
+val mem : a:'a -> l:list 'a -> option (Mem 'a a l)
+let rec mem (a : 'a) (l: list 'a) : option (Mem 'a a l) =
+  match l with
+  | [] -> None
+  | h::t when h=a -> Some(Mem_hd a t)
+  | h::t -> (match mem a t with
+               | None -> None
+			   | Some(m) -> Some(Mem_tl a h t m))
+
+val memSubstrate : q:query -> s:substrate -> option (Mem q s)
+  (* Rk: using _S instead of s in the type declaration confuses F* *)
+let memSubstrate q _S = mem q _S
+  (* Rk: does not accept : let memSubstrate = mem which is essentially the same *)
+  
+val memInfostrate : i:infon -> is:infostrate -> option (Mem i is)
+let memInfostrate i _I = mem i _I
 
 
-type In :: 'a::* => 'a => list 'a => P (* Inductive definition of list membership in a constructive style *)
-
+(* Intuition:                                                 *)
+(* MkPrefix [p1;...;pn] i (p1 said (p2 said ... (pn said i))) *)
 type MkPrefix :: list infon => infon => infon => P =
   | MkPrefix_Nil : i:infon -> MkPrefix [] i i
   | MkPrefix_Cons : p:infon -> ps:list infon -> i:infon -> i':infon 
                    -> MkPrefix ps i i'
                    -> MkPrefix (p::ps) i (Said p i')
 
-type entails :: substrate => infostrate => infon => P =
-  | Entails_Emp : S:substrate -> I:infostrate -> entails S I Empty
+(* Intuition:                                                    *) 
+(* mkPrefix [p1;...;pn] i = ( (p1 said (... pn said i)), proof ) *)
+val mkPrefix: pref:prefix -> i:infon -> (i':infon * dummy:(MkPrefix pref i i'){pref=[] => i=i'})
+let rec mkPrefix pref i =
+  (match pref with
+     | [] -> (i, MkPrefix_Nil i)
+     | h::t -> let (j, m) = mkPrefix t i in
+	             ((Said h j), MkPrefix_Cons h t i j m))				   
 
-  | Entails_Hyp_Substrate : S:substrate -> I:infostrate -> q:query 
-                 -> In q S  (* Eventually, we get a signature from the DB about this fact *)
-                 -> entails S I (AsInfon q)
 
-  | Entails_And_Intro : S:substrate -> I:infostrate 
+(***********************)
+(* Inductive judgments *)
+(***********************) 
+
+(*type types :: varDecl => ? => typ => P =*)
+
+type entails :: substrate => infostrate => varDecl => infon => P =
+  | Entails_Emp : S:substrate -> I:infostrate -> G:varDecl
+               -> pref: prefix
+			   -> result: infon
+			   -> MkPrefix pref Empty result
+			   -> entails S I G result
+
+  | Entails_Hyp_Knowledge : S:substrate -> I:infostrate -> G:varDecl
+                          -> i:infon
+						  -> Mem i I
+						  -> entails S I G i
+						  
+  | Entails_Hyp_Substrate : S:substrate -> I:infostrate -> G:varDecl
+                          -> q:query 
+                          -> Mem q S  
+						  (* Eventually, we get a signature from the DB about this fact *)
+                          -> entails S I G (AsInfon q)
+
+  (* Q: here order of G matters; make sure that's all right; I think so *)
+  | Entails_Q_Intro : S:substrate -> I:infostrate -> G:varDecl
+                    -> x:var -> i:infon -> i':infon
+					-> result:infon
+					-> pref:prefix
+			        (*-> MkPrefix pref (Forall x i) result *) (* TODO?? *)
+					-> MkPrefix pref i i'
+			        -> entails S I (x::G) i'
+					-> entails S I G result
+				 
+  | Entails_And_Intro : S:substrate -> I:infostrate -> G:varDecl
                      -> i:infon -> i':infon
                      -> j:infon -> j':infon 
                      -> result:infon
-                     -> pref: list infon
+                     -> pref: prefix
                      -> MkPrefix pref (And i j) result
                      -> MkPrefix pref i i'
                      -> MkPrefix pref j j'
-                     -> entails S I i' 
-                     -> entails S I j' 
-                     -> entails S I result
+                     -> entails S I G i' 
+                     -> entails S I G j' 
+                     -> entails S I G result
 
-  | Entails_And_Elim1 : S:substrate -> I:infostrate
+  | Entails_And_Elim1 : S:substrate -> I:infostrate -> G:varDecl
      -> i : infon -> i': infon
      -> j : infon
      -> pref : list infon 
      -> hyp : infon
      -> MkPrefix pref (And i j) hyp
      -> MkPrefix pref i i'
-     -> entails S I hyp
-     -> entails S I i'
+     -> entails S I G hyp
+     -> entails S I G i'
+	 
+  | Entails_W_Imp_Intro : S:substrate -> I:infostrate -> G:varDecl 
+                      -> i:infon
+                      -> j:infon -> j':infon 
+                      -> result:infon
+                      -> pref: list infon
+                      -> MkPrefix pref (Implies i j) result
+                      -> MkPrefix pref j j'
+                      -> entails S I G j' 
+                      -> entails S I G result
 
+					  
+(*
+type Typing :: varDecl => term => typ => P =
+   | Typing_var : g:varDecl -> x:var -> t:typ -> Mem (x,t) g -> Typing g (VarTerm x) t
+*)
+(* val subst: i:infon -> x:var -> u:term -> (i':infon * Subst i x u i') *)
+(* let subst i x u = raise "todo" *)
 
-val checkSubstrate : S:substrate -> q:query -> option (In q S)
-(* Left unimplemented for now *)
+type Subst :: infon => var => term => infon => P = 
+   | Subst_admit : i:infon -> x:var -> t:term -> i':infon -> Subst i x t i'
 
-type prefix = list infon
+val subst: i:infon -> x:var -> u:term -> (i':infon * Subst i x u i')
+let subst i x u = raise "todo"
 
-val mkPrefix: pref:prefix -> i:infon -> (i':infon * dummy:(MkPrefix pref i i'){pref=[] => i=i'})
-let rec mkPrefix pref i =
-  (match pref with
-     | [] -> (i, MkPrefix_Nil i)
-     | h::t -> let (j, m) = mkPrefix t i in
-	             ((Said h j), MkPrefix_Cons h t i j m))
+(************************)
+(* Derivation algorithm *)
+(************************) 
 
-val doDerive: S:substrate -> I:infostrate -> pref:prefix -> i:infon 
-           -> option (i':infon * MkPrefix pref i i' * entails S I i')
-let rec doDerive _S _I pref i = match i with 
-  | Empty -> 
-      (match pref with 
-         | [] -> let (j, m) = mkPrefix pref i in
-		 (* if unable to make F* prove sth, put in a runtime check *)
-			     (* if j = Empty then *)
-                   Some((j, m, Entails_Emp _S _I))
-				  (* else raise "stupid F*" *)
-         | _ -> None)
+val doDerive: S:substrate -> I:infostrate -> G:varDecl 
+           -> pref:prefix -> i:infon 
+           -> option (i':infon * MkPrefix pref i i' * entails S I G i')
+let rec doDerive _S _I _G pref inf = 
+  let memInfostrate_inf = memInfostrate inf _I in
+  match inf with 
+  | Empty -> let (j, m) = mkPrefix pref inf in
+		              (* if unable to make F* prove sth, put in a runtime check *)
+			          (* if j = Empty then *)
+                   Some((j, m, 
+				         Entails_Emp _S _I _G pref j m))
+				      (* else raise "stupid F*" *)
 
+  | i when ((pref = []) && (not (memInfostrate_inf = None))) ->
+      let (j, m) = mkPrefix pref inf in
+	  (match memInfostrate_inf with
+	     | None -> raise "assert false"
+         | Some mis -> Some((j, m, Entails_Hyp_Knowledge _S _I _G i mis)))
+		 
   | AsInfon q -> 
       (match pref with
-         | [] -> let (j, m) = mkPrefix pref i in
-             (match checkSubstrate _S q with 
+         | [] -> let (j, m) = mkPrefix pref inf in
+             (match memSubstrate q _S with 
                 | None -> None
-                | Some pf -> Some ((j, m, Entails_Hyp_Substrate _S _I q pf)))
+                | Some pf -> Some ((j, m, Entails_Hyp_Substrate _S _I _G q pf)))
          | _ -> None)
 
-  | And i j -> None (*Some((,,))*)
+  | Forall x i ->
+      (match doDerive _S _I (x::_G) pref i with
+	     | None -> None
+		 | Some((i', mi, ei)) -> 
+             let (j, m) = mkPrefix pref inf in
+	         Some((j, m, Entails_Q_Intro _S _I _G x i i' j pref (*m*) mi ei)))
+	 
+  | And i j ->
+      (match (doDerive _S _I _G pref i, doDerive _S _I _G pref j) with
+	     | (None, _) -> None
+	     | (_, None) -> None
+	     | (Some((i', mi, ei)), Some((j', mj, ej))) -> 
+		      let (a, m) = mkPrefix pref inf in
+		      Some((a, m,
+                    Entails_And_Intro _S _I _G i i' j j' a pref m mi mj ei ej)))
+					
+  | Implies i j ->
+      (match doDerive _S _I _G pref j with
+	     | None -> None
+         | Some((j', mj, ej)) ->
+             let (a, m) = mkPrefix pref inf in
+			 Some((a, m,
+			       Entails_W_Imp_Intro _S _I _G i j j' a pref m mj ej)))
+	  
+
       
